\documentclass[12pt]{article}
\pagestyle{empty}

\everymath{\displaystyle}

\usepackage[a4paper, margin=0.75in]{geometry}
\usepackage{amssymb}

\newcommand{\tab}{\hspace*{0.55in}}
\renewcommand{\labelenumi}{(\roman{enumi})}

\begin{document}
\begin{enumerate}
    \item
    Let, $ f(x) = e^x $ \\
    $ \therefore f(x+h) = e^{x+h}$ \\
    From the definition of derivatives, $ f'(x) = \lim_{h \to 0} \frac{f(x+h) - f(x)}{h} $ \\
    $ \therefore f'(x) = \lim_{h \to 0} \frac{e^{x+h} - e^x}{h} $ \\
    \tab $ = \lim_{h \to 0} \frac{e^x(e^h -1)}{h} $ \\
    % TODO: Why the \quad tab not working?
    % TODO: How the get the better alignment, where all equal signs are aligned perfectly?
    \tab $ = e^x \cdot \lim_{h \to 0} \frac{1}{h} \left\{ \left( 1 + \frac{h}{1!} + \frac{h^2}{2!} + \frac{h^3}{3!} + \ldots \right) - 1 \right\} $ \\
    \tab $ = e^x \cdot \lim_{h \to 0} \left( 1 + \frac{h}{2!} + \frac{h^2}{3!} + \ldots \right) $ \\
    \tab $ = e^x $

    \item
    Let, $ f(x) = a^x $ \\
    $ \therefore f'(x) = \lim_{h \to 0} \frac{a^{x+h} - a^x}{h} $ \\
    \tab $ = \lim_{h \to 0} \frac{a^x (a^h - 1)}{h}$ \\
    \tab $ = a^x \cdot \lim_{h \to 0} \frac{1}{h} \left\{ \left( 1 + \frac{h}{1!} \ln a + \frac{h^2}{2!} (\ln a)^2 + \ldots \right) - 1 \right\}$ \\
    \tab $ = a^x \cdot \lim_{h \to 0} \left( \ln a + \frac{h}{2!} (\ln a)^2 + \ldots \right) $ \\
    \tab $ = a^x \ln a $

    \item
    Let, $ f(x) = \ln x $ \\
    $ \therefore f'(x) = \lim_{h \to 0} \frac{\ln(x+h)-\ln x}{h} $ \\
    \tab $ = \lim_{h \to 0} \frac{\ln \frac{x+h}{x}}{h} $ \\
    \tab $ = \lim_{h \to 0} \frac{1}{h} \ln \left( 1 + \frac{h}{x} \right) $ \\
    \tab $ = \lim_{h \to 0} \frac{1}{h} \left( \frac{h}{x} - \frac{1}{2} \cdot \frac{h^2}{x^2} + \frac{1}{3} \cdot \frac{h^3}{x^3} - \ldots \right) $ \\
    \tab $ = \lim_{h \to 0} \left( \frac{1}{x} - \frac{h}{2x^2} + \frac{h^2}{3x^3} - \ldots \right)$ \\
    \tab $ = \frac{1}{x} $

    \item
    Let, $ f(x) = \sin x $ \\
    $ \therefore f'(x) = \lim_{h \to 0} \frac{\sin(x+h) - \sin x}{h} $ \\
    \tab $ = \lim_{h \to 0} \frac{2 \cos\left(x + \frac{h}{2}\right) \sin \frac{h}{2}}{h} $ \\
    \tab $ = \lim_{h \to 0} \left\{ \cos\left( x + \frac{h}{2} \right) \cdot \frac{\sin \frac{h}{2}}{\frac{h}{2}} \right\} $ \\
    \tab $ = \lim_{h \to 0} \left\{ \cos \left( x + \frac{h}{2} \right) \right\} \cdot \lim_{\frac{h}{2} \to 0} \left\{ \frac{\sin \frac{h}{2}}{\frac{h}{2}} \right\} $ \\
    \tab $ = \cos x \cdot 1 $ \\
    \tab $ = \cos x $
\end{enumerate}
\end{document}
